Made the I2MP/Examples tests work for Merged, and implemented debugging/printing helper functions as well. Added tags for values in Transitional.

I2MP/Examples/Helper.v
@@ -38,7 +38,7 @@ Instance showInt : Show int :=
 
 Instance showWord {k : nat} : Show (word k) :=
   {
-  show m := show (fintype.nat_of_ord (val m))
+  show m := show (ssrint.absz (int_of_word m)) (*fintype.nat_of_ord (eqtype.val m)*)
   }.
 
 (* Instance showRegInt : Show (Types.reg mt) := *)
@@ -57,8 +57,12 @@ Instance showValue : Show value :=
   end
 }.
 
+Instance showTvalue : Show tvalue :=
+ {
+  show tv := show (val tv) (* TODO *)
+}.
 
-Instance showRegInter : Show (Intermediate.Register.t) :=
+Instance showRegInter : Show (Register.t) :=
  {
  show r :=   foldl (fun acc '(n,v) =>
            acc ++ (show n) ++ " : "
@@ -118,25 +122,45 @@ Instance show_trans : Show Transitional.instr :=
   {| show :=
        fun i =>
          match (i:Transitional.instr) with
-           | Transitional.TrNop => "INop"
-           | Transitional.TrLabel lbl => "ILabel " ++ (show lbl)
-           | Transitional.TrConst v r => "IConst " ++ (show v) ++ " " ++ (show r)
-           | Transitional.TrMov r1 r2 => "IMov " ++ (show r1) ++ " " ++ (show r2)
-           | Transitional.TrBinOp op r1 r2 r3 => "IBinop " ++ (show op)
+           | Transitional.TrNop => "TrNop"
+           | Transitional.TrLabel lbl => "TrLabel " ++ (show lbl)
+           | Transitional.TrConst v r => "TrConst " ++ (show v) ++ " " ++ (show r)
+           | Transitional.TrMov r1 r2 => "TrMov " ++ (show r1) ++ " " ++ (show r2)
+           | Transitional.TrBinOp op r1 r2 r3 => "TrBinop " ++ (show op)
                                             ++ " " ++ (show r1)
                                             ++ " " ++ (show r2)
                                             ++ " " ++ (show r3)
-           | Transitional.TrLoad r1 r2 => "ILoad " ++ (show r1) ++ " " ++ (show r2)
-           | Transitional.TrStore r1 r2 => "IStore " ++ (show r1) ++ " " ++ (show r2)
-           | Transitional.TrAlloc r1 r2 => "IAlloc " ++ (show r1) ++ " " ++ (show r2)
-           | Transitional.TrBnz r l => "IBnz " ++ (show r) ++ " " ++ (show l)
-           | Transitional.TrJump r => "IJump " ++ (show r)
-           | Transitional.TrJalNat l => "IJalNat " ++ (show l)
-           | Transitional.TrJalProc l => "IJalProc " ++ (show l)
-           | Transitional.TrHalt => "IHalt"
+           | Transitional.TrLoad r1 r2 => "TrLoad " ++ (show r1) ++ " " ++ (show r2)
+           | Transitional.TrStore r1 r2 => "TrStore " ++ (show r1) ++ " " ++ (show r2)
+           | Transitional.TrAlloc r1 r2 => "TrAlloc " ++ (show r1) ++ " " ++ (show r2)
+           | Transitional.TrBnz r l => "TrBnz " ++ (show r) ++ " " ++ (show l)
+           | Transitional.TrJump r => "TrJump " ++ (show r)
+           | Transitional.TrJalNat l => "TrJalNat " ++ (show l)
+           | Transitional.TrJalProc l => "TrJalProc " ++ (show l)
+           | Transitional.TrHalt => "TrHalt"
          end
   |}.
 
+Instance show_intermediate : Show Machine.instr :=
+  {
+    show i :=
+      match i with
+      | INop => "INop"
+      | ILabel l => "ILabel " ++ (show l)
+      | IConst im r => "IConst " ++ (show im) ++ " " ++ (show r)
+      | IMov r1 r2 => "IMov " ++ (show r1) ++ " " ++ (show r2)
+      | IBinOp b r1 r2 r3 => "IBinop " ++ (show b) ++ " " ++ (show r1) ++ " " ++ (show r2) ++ " " ++ (show r3)
+      | ILoad  r1 r2 => "ILoad " ++ (show r1) ++ " " ++ (show r2)
+      | IStore  r1 r2 => "IStore " ++ (show r1) ++ " " ++ (show r2)
+      | IAlloc  r1 r2 => "IAlloc " ++ (show r1) ++ " " ++ (show r2)
+      | IBnz r l => "IBnz " ++ (show r) ++ " " ++ (show l)
+      | IJump r => "IJump " ++ (show r)
+      | IJal l => "IJal " ++ (show l)
+      | ICall c p => "ICall " ++ (show c) ++ " " ++ (show p)
+      | IReturn => "IReturn"
+      | IHalt => "IHalt"
+      end
+  }.
 
 Definition show_nmap { A :Type} `{_ : Show A} (m : (NMap A)) : string :=
   List.fold_left
@@ -149,12 +173,12 @@ Definition show_nmap { A :Type} `{_ : Show A} (m : (NMap A)) : string :=
 
 
 
-Instance show_dummymemtag : Show Transitional.mem_tag :=
+Instance show_dummymemtag : Show LRC.mem_tag :=
  {
   show mt := ""
 }.
 
-Instance show_seq : Show (list (Transitional.instr * Transitional.mem_tag)) :=
+Instance show_seq  { A :Type} `{_ : Show A} : Show (list A) :=
 {
   show l := let fix show_aux l := match l with 
     | [] => ""
@@ -164,6 +188,16 @@ Instance show_seq : Show (list (Transitional.instr * Transitional.mem_tag)) :=
 }.
 
 Instance show_code : Show Transitional.code :=
+ {
+  show c := show_nmap c
+}.
+
+Instance show_intermediate_code_aux : Show (NMap code) :=
+ {
+  show c := show_nmap c
+}.
+
+Instance show_intermediate_code : Show (NMap (NMap code)) :=
  {
   show c := show_nmap c
 }.
@@ -190,3 +224,211 @@ Definition compile_and_show (p: Source.program) :=
 (*     | Some st' => fstate_to_unit (print_regs st' 6 fstate0) *)
 (*     end *)
 (* . *)
+
+Require Import MicroPolicies.Merged MicroPolicies.Symbolic Int32.
+
+
+Instance showRegisterTag : Show (Symbolic.tag_type LRC.lrc_tags Symbolic.R) :=
+ {
+  show rt := match rt with LRC.Ret n => "Ret " ++ (show n) | LRC.Other => "Other" end
+}.
+
+
+Instance showMemoryTag : Show (Symbolic.tag_type LRC.lrc_tags Symbolic.M) :=
+ {
+   show mt := (match LRC.vtag mt with | LRC.Ret n => ("Ret " ++ (show n)) | LRC.Other => "Other" end)
+               ++ " ; c=" ++ (show (LRC.color mt) ++
+              (match (LRC.entry mt) with | None => " ; no entry" | Some e => " ; entry = " ++ (show e) end))
+ }.
+
+
+Definition tab := String (Ascii.ascii_of_pos 9) ""%string.
+
+Definition register_of_nat (n : nat) : string :=
+  match n with  
+    | 0  => "R_ONE"
+    | 1  => "R_COM"
+    | 2  => "R_AUX1"
+    | 3  => "R_AUX2"
+    | 4  => "R_RA "
+    | 5  => "R_SP "
+    | 6  => "R_ARG"
+    | 16 => "R_SC_RET"
+    | 17 => "R_SC_ARG1"
+    | 18 => "R_SC_ARG2"
+    | 19 => "R_SC_ARG3"
+    | _  => "NOT A REG"
+  end.
+
+Instance showRegister : Show (register) :=
+  {
+    show r := register_of_nat (Intermediate.Machine.Intermediate.Register.to_nat r)
+  }.
+
+Instance showSysreg : Show (Merged.sys_reg) :=
+  {
+    show r := register_of_nat (Merged.to_nat_bis (inr r))
+  }.
+
+
+Instance showRegSysreg : Show (register + Merged.sys_reg) :=
+  {
+    show r :=
+      match r with
+        | inl r => show r | inr r => show r
+      end
+  }.
+
+Instance showRegisters : Show (@Merged.registers concrete_int_32_mt) :=
+ {
+ show r :=   foldl (fun acc '(n,v) =>
+           acc ++ (register_of_nat ( n)) ++ " : " ++ tab 
+               ++ (show (MicroPolicies.Types.vala v)) ++ " @ "
+               ++ (show (MicroPolicies.Types.taga v)) ++ newline)
+        "" (Maps.elementsm r)
+ }.
+
+Definition elementsm {A: Type} {k : nat} : {fmap (word k) -> A} -> list ((word k) * A).
+Proof.
+     exact (@FMap.fmval (word_ordType k) A _)
+  ||
+     idtac "ExStructures 0.1 legacy definition inactive";
+     exact (@FMap.fmval (word_ordType k) A).
+Defined.
+
+Instance showMemory : Show (@Merged.memory concrete_int_32_mt) :=
+ {
+ show m :=   (foldl (fun acc '(n,v) =>
+           acc ++ (show n) ++ " : "
+               ++ (show (MicroPolicies.Types.vala v)) ++ " @ "
+               ++ (show (MicroPolicies.Types.taga v)) ++ " | ")
+        "" (elementsm m))
+ }.
+
+Instance showState : Show (Merged.state) :=
+  {
+    show st :=
+      let n := match (MicroPolicies.Types.taga (Merged.pc st)) with LRC.Level m => m end in
+      "---------------------" ++ newline ++
+   "Memory: " ++ newline ++ (show (Merged.mem st)) ++ newline ++ "Registers: " ++ newline ++ (show (Merged.regs st )) ++ newline ++ "pc: " ++ show (MicroPolicies.Types.vala (Merged.pc st)) ++ "; level: " ++ show (ssrint.Posz n) ++ newline ++ "---------------------" ++ newline
+  }.
+
+
+Instance showMergedInstr : Show (@Merged.instr concrete_int_32_mt) :=
+  {
+    show i := match i with              
+  | MrNop     => "MrNop"
+  | MrConst i r  => "MrConst " ++ (show i) ++ " " ++ (show r)
+  | MrMov r1 r2   => "MrMov " ++ (show r1) ++ " " ++ (show r2)
+  | MrBinop b r1 r2 r3 => "MrBinop " ++ (show b) ++ " " ++ (show r1) ++ " " ++ (show r2) ++ " " ++ (show r3)
+  | MrLoad r1 r2  => "MrLoad " ++ (show r1) ++ " " ++ (show r2)
+  | MrStore r1 r2 => "MrStore "++ (show r1) ++ " " ++ (show r2)
+  | MrJump r   => "MrJump " ++ (show r)
+  | MrBnz r l   => "MrBnz " ++ (show r) ++ " " ++ (show l)
+  | MrJal l    => "MrJal " ++ (show l)
+  | MrHalt    => "MrHalt "
+  | MrLabel l  => "MrLabel " ++ (show l)
+  end
+  }.
+  
+Instance showMergedCode : Show (@Merged.code concrete_int_32_mt) :=
+  {
+    show c := "Merged code: " ++ (show (size c)) ++ " lines." ++ newline ++
+   (let (_,s) := (foldl (fun (acc:(nat*string)) (p:(instr*LRC.mem_tag)) =>
+                           let (n, a) := acc in let (i, t) := p in
+                           (n+1, a ++ (show n) ++ " " ++ (show i) ++ " @ " ++ (show t) ++ newline)
+                 ) (0,"") c) in s)
+  }.
+
+Definition printer {T : Type} (_:string) (v:T) : T := v.
+
+Extract Constant printer => "(fun s v -> (List.fold_left (fun acc c -> print_char c; acc) () s); print_newline () ; v)". 
+
+Fixpoint execN_and_show (n: nat) (cde: Merged.code) (st: state) : option Z + nat :=
+  printer (show st)
+  match n with
+  | O => inr 3
+  | S n' =>
+    match Merged.eval_step cde st with
+    | None => (inl (
+             do! w <- (regs st (Intermediate.Machine.Intermediate.Register.to_nat R_COM));
+             Some (Symbolic.convert (word.int_of_word (MicroPolicies.Types.vala w)))))
+    | Some (st', _) => execN_and_show n' cde st'
+    end
+  end.
+
+Fixpoint execN_pc (n: nat) (cde: Merged.code) (st: state) : option Z + nat :=
+  printer (show (Types.vala (pc st)) ++ " ; ")
+  match n with
+  | O => inr 3
+  | S n' =>
+    match Merged.eval_step cde st with
+    | None => (inl (
+             do! w <- (@regs concrete_int_32_mt st (Intermediate.Machine.Intermediate.Register.to_nat R_COM));
+             Some (Symbolic.convert (word.int_of_word (MicroPolicies.Types.vala w)))))
+    | Some (st', _) => execN_pc n' cde st'
+    end
+  end.
+
+(* execute interemdiary code and lists out the progam counters *)
+Fixpoint execN_pc_inter (n: nat) (G: Intermediate.GlobalEnv.global_env) (st: Intermediate.CS.CS.state) : string :=
+  let '(_,_,r,pc) := st in
+  (show pc) ++ " | R_RA : " ++ (show (r 4)) ++ newline ++
+  match n with
+  | O => "out of fuel"
+  | S n' =>
+    match Intermediate.CS.CS.eval_step G st with
+    | None =>
+      let '(_, _, regs, _) := st in
+      match Intermediate.Machine.Intermediate.Register.get R_COM regs with
+      | Int i => ("result : " ++ (show i))
+      | _ => "error"
+      end
+    | Some (_, st') => execN_pc_inter n' G st'
+    end
+  end.
+
+Definition run_inter_and_show_pc (n : nat) (p : Intermediate.program) : string :=
+  let G := Intermediate.GlobalEnv.prepare_global_env p in
+  let st := Intermediate.CS.CS.initial_machine_state p in
+  execN_pc_inter n G st.
+
+From CoqUtils Require Import hseq word.
+
+
+Definition run_and_show_merged (cd:code) mem0 fuel :=
+  let default_reg := {| MicroPolicies.Types.vala := (word_of_nat 0) ; MicroPolicies.Types.taga := (LRC.Other) |} in
+  let reg0 := [fmap (0, default_reg) ;
+               (1, default_reg) ;
+               (2, default_reg) ;
+               (3, default_reg) ;
+               (4, {| MicroPolicies.Types.vala := (word_of_nat (1 + size cd)) ; MicroPolicies.Types.taga := (LRC.Other) |}) ;
+               (5, default_reg) ;
+               (6, default_reg) ;
+               (16,default_reg) ;
+               (17,default_reg) ;
+               (18,default_reg) ;
+               (19,default_reg) ] in
+  let pctag := LRC.build_tpc 0 in
+  let pc := {| MicroPolicies.Types.vala := (word_of_nat 0) ; MicroPolicies.Types.taga := pctag |} in
+  let st := {|mem := mem0 ; regs := reg0 ; pc := pc|} in
+  printer (show cd)
+  execN_and_show fuel cd st.
+
+Definition compile_and_run_and_show_from_source_merged (mt : Types.machine_types) := 
+fun (p : Source.program) (fuel : nat) =>
+match Compiler.compile_program p with
+| Some compiled_p =>
+    printer (show (Intermediate.prog_procedures compiled_p))
+    printer (show (pre_linearize compiled_p)) 
+    printer ( "intermediary pc : " ++ newline)
+    printer (run_inter_and_show_pc fuel compiled_p)
+    (*
+    printer (show (transitional_to_merged (pre_linearize compiled_p)))*)
+    match @run_and_show_merged (transitional_to_merged compiled_p (pre_linearize compiled_p)) (inital_memory compiled_p) fuel with
+    | inl (Some n) => print_ocaml_int (z2int n)
+    | inl None => print_error ocaml_int_1
+    | inr n => print_error (nat2int n)
+    end
+| None => print_error ocaml_int_0
+end.
