MicroPolicies/Merged.v
@@ -9,15 +9,20 @@ Require Import Transitional.
 Require Import MicroPolicies.Utils MicroPolicies.LRC MicroPolicies.Symbolic Intermediate.Machine.
 Require Import CompCert.Events.
 
+
+Require Import Source.Language S2I.Compiler.
+Require Export Extraction.Definitions.
+
+
 Set Implicit Arguments.
 Unset Strict Implicit.
 Unset Printing Implicit Defensive.
 Import DoNotation.
 
 
-Context {mt : machine_types} {ops : machine_ops mt}.
+Section WithClasses.
 
-Search (sum).
+Context {mt : machine_types} {ops : machine_ops mt}.
 
 (* system call registers *)
 Inductive sys_reg : Set :=
@@ -41,13 +46,6 @@ Variant instr :=
 | MrHalt : instr.
 
 
-(* Memory model and definition are the same as defined in LRC.v *) 
-(*
-Notation state := (@Symbolic.state mt sym_lrc).
-Notation State := (@Symbolic.State mt sym_lrc).
- *)
-
-
 Definition nat_of_word {k : nat} (w : (word k)) : nat := (ssrint.absz (word.int_of_word w)).
 Definition word_of_nat {k : nat} (n : nat) : (word k) := (word.as_word (ssrint.Posz n)).
 
@@ -56,8 +54,8 @@ Local Notation tag_type := (Symbolic.tag_type lrc_tags).
 Local Notation word := (mword mt).
 Let atom := (Types.atom word).
 
-Local Notation memory := {fmap word -> atom (tag_type Symbolic.M)}.
-Local Notation registers := {fmap nat -> (atom (tag_type Symbolic.R))}%type.
+Definition memory := {fmap word -> atom (tag_type Symbolic.M)}.
+Definition registers := {fmap nat -> (atom (tag_type Symbolic.R))}%type.
 
 Notation to_nat := Intermediate.Machine.Intermediate.Register.to_nat.
 Definition from_nat (n : nat) : register :=
@@ -76,10 +74,10 @@ Definition to_nat_bis (r : register + sys_reg) : nat :=
     | inl r => to_nat r
     | inr r =>
         match r with
-          R_SC_RET => 7
-        | R_SC_ARG1 => 8
-        | R_SC_ARG2 => 9
-        | R_SC_ARG3 => 10
+          R_SC_RET => 16
+        | R_SC_ARG1 => 17
+        | R_SC_ARG2 => 18
+        | R_SC_ARG3 => 19
         end
 end.
 
@@ -92,8 +90,6 @@ Record state := State {
 }.
 
 Notation state_ev := (state * option event)%type.
-
-(* Notation update := (@Symbolic.update mt).*)
 
 Inductive update :=
   | RegWrite : (register + sys_reg) -> word -> update
@@ -112,22 +108,7 @@ Definition executing (cde : code) (pc : mword mt) (i : instr) : Prop :=
   let off := Symbolic.convert (word.int_of_word pc) in
   (off >= 0) % Z /\ nth_error cde (Z.to_nat off) = Some (i,tg).
 
-(*
-Definition outputs (op : instr) : seq Symbolic.tag_kind :=
-  match op with    
-  | MrNop     => [:: ]
-  | MrConst _ _  => [:: Symbolic.R]
-  | MrMov _ _   => [:: Symbolic.R;Symbolic.R]
-  | MrBinop _ _ _ _ => [:: Symbolic.R;Symbolic.R;Symbolic.R]
-  | MrLoad _ _  => [:: Symbolic.R;Symbolic.M;Symbolic.R]
-  | MrStore _ _ => [:: Symbolic.R;Symbolic.R;Symbolic.M]
-  | MrJump _   => [:: Symbolic.R]
-  | MrBnz _ _   => [:: Symbolic.R]
-  | MrJal _    => [:: Symbolic.R]
-  | MrHalt    => [::]
-                  
-  | MrLabel _  => [::]
-  end.*)
+
 Definition outputs := Symbolic.outputs.
 Definition inputs := outputs.
 
@@ -253,12 +234,12 @@ Fixpoint next_state_do_updates (st : state) (tks : seq Symbolic.tag_kind)
   end.
 
 (* pc' is the new, target pc *)
-Definition next_state_updates_and_pc (st : state) 
+Definition next_state_updates_and_pc (cde : code) (st : state) 
   (op : opcode)
   (iv : ivec op)
   (updts : seq update)
   (pc' : word) : option state_ev :=
-  let tni := match mem st pc' with | None => None | Some ni => Some (taga ni) end in
+  let tni := match ((nth_error cde (nat_of_word pc'))) with | None => None | Some (_,t) => Some (t) end in
   let k :=
     (fun (ov_ev:((ovec op) * (option event))) => let (ov,ev) := ov_ev in
        do! st' <- next_state_do_updates st (tr ov) updts;
@@ -266,23 +247,23 @@ Definition next_state_updates_and_pc (st : state)
     ) in
   next_state st iv tni k.
 
-Definition next_state_updates (st : state) 
+Definition next_state_updates (cde : code) (st : state) 
   (op : opcode)
   (iv : ivec op)
   (updts : seq update) : option state_ev :=
-  next_state_updates_and_pc st iv updts (word_of_nat (nat_of_word (vala (pc st))).+1).
+  next_state_updates_and_pc cde st iv updts (word_of_nat (nat_of_word (vala (pc st))).+1).
 
 Fixpoint find_label_aux (cde : code) (l : label) (n : nat) : option nat :=
   match cde with
   | nil => None
-  | cons (MrLabel l, _) ccde => Some n
+  | cons (MrLabel l2, _) ccde => if (eqn l l2) then (Some n) else find_label_aux ccde l (n+1)
   | cons _ ccde => find_label_aux ccde l (n+1)
   end.
 
 (* TODO : check for potential off-by-one error *)
 (* find the word w of a pc pointing to the label l in cde *)
-Fixpoint find_label (cde : code) (l : label) : option word :=
-  do! res <- find_label_aux cde l 0; Some (word_of_nat res).
+Definition find_label (cde : code) (l : label) : option nat :=
+  find_label_aux cde l 0.
 
 Definition binop_of_binop (b : binop) : Types.binop :=
   match b with
@@ -293,14 +274,15 @@ Definition binop_of_binop (b : binop) : Types.binop :=
   | Leq => LEQ
   end.
 
-Definition alloc_fun (st : state) : option state :=
+Definition alloc_fun (cde : code) (st : state) : option state :=
   (* TL TODO: Rely on the fact that it set implem is a sorted list, kinda fishy *)
-  let max_addr := last (as_word (ssrint.Posz 0)) (domm (mem st)) (* (@as_word (word_size mt) (ssrint.Posz 0)) *) in (* TODO : what to actually put here? *)
+  let max_addr := last (as_word (ssrint.Posz 0)) (domm (mem st)) in (* TODO : what to actually put here? *)
   do! ra_val <- regs st (to_nat R_RA);
   let next_pc := (vala ra_val)@(taga (pc st)) in
   (* TL TODO: Is using return address to compute calling component safe? *)
-  do! ra_atom <- mem st (vala ra_val);
-  let current_c := (color (taga ra_atom)) in
+  (*do! ra_atom <- mem st (vala ra_val);*)
+  do! current_instr <- nth_error cde (nat_of_word (vala (pc st)));
+  let current_c := (color (snd current_instr)) in
   (* create the new bloc *)
   let atom : matom := (word.as_word (ssrint.Posz 0))@(def_mem_tag current_c) in
   do! size <- regs st (to_nat_bis (inr R_SC_ARG1));
@@ -327,20 +309,20 @@ Inductive step (cde : code) (st st' : state) (ev : option event) : Prop :=
     (PC   : mem pc = Some i@ti)
     (INST : executing cde pc MrNop),
     let iv : ivec NOP := IVec tpc ti ([hseq] : hseq _ (inputs NOP)) in forall
-    (NEXT : next_state_updates st iv [:: ] = Some (st', ev)),    step cde st st' ev
+    (NEXT : next_state_updates cde st iv [:: ] = Some (st', ev)),    step cde st st' ev
 | step_label : forall mem reg pc tpc i ti l
     (ST   : st = State mem reg pc@tpc)
     (PC   : mem pc = Some i@ti)
     (INST : executing cde pc (MrLabel l)),
     let iv : ivec NOP := IVec tpc ti ([hseq] : hseq _ (inputs NOP)) in forall
-    (NEXT : next_state_updates st iv [:: ] = Some (st', ev)),    step cde st st' ev
+    (NEXT : next_state_updates cde st iv [:: ] = Some (st', ev)),    step cde st st' ev
 | step_const : forall mem reg pc tpc i ti n r old (told : tag_type Symbolic.R) 
     (ST   : st = State mem reg pc@tpc)
     (PC   : mem pc = Some i@ti)
     (INST : executing cde pc (MrConst n r))
     (OLD  : reg (to_nat r) = Some old@told),
     let mvec := IVec tpc ti ([hseq told] : hseq _ (inputs CONST)) in forall
-    (NEXT : next_state_updates st mvec [:: RegWrite (inl r) (swcast n)] = Some (st', ev)),   step cde st st' ev
+    (NEXT : next_state_updates cde st mvec [:: RegWrite (inl r) (swcast n)] = Some (st', ev)),   step cde st st' ev
 | step_mov : forall mem reg pc tpc i ti r1 w1 t1 r2 old told
     (ST   : st = State mem reg pc@tpc)
     (PC   : mem pc = Some i@ti)
@@ -348,7 +330,7 @@ Inductive step (cde : code) (st st' : state) (ev : option event) : Prop :=
     (R1W  : reg (to_nat_bis r1) = Some w1@t1)
     (OLD  : reg (to_nat_bis r2) = Some old@told),
     let mvec := IVec tpc ti ([hseq t1; told] : hseq _ (inputs MOV)) in forall
-    (NEXT : next_state_updates st mvec [:: RegRead r1 ; RegWrite r2 w1 ] = Some (st', ev)),   step cde st st' ev
+    (NEXT : next_state_updates cde st mvec [:: RegRead r1 ; RegWrite r2 w1 ] = Some (st', ev)),   step cde st st' ev
 | step_binop : forall mem reg pc tpc i ti op r1 r2 r3 w1 w2 t1 t2 old told
     (ST   : st = State mem reg pc@tpc)
     (PC   : mem pc = Some i@ti)
@@ -357,7 +339,7 @@ Inductive step (cde : code) (st st' : state) (ev : option event) : Prop :=
     (R2W  : reg (to_nat r2) = Some w2@t2)
     (OLD  : reg (to_nat r3) = Some old@told),
     let mvec := IVec tpc ti ([hseq t1; t2; told] : hseq _ (inputs (BINOP (binop_of_binop op)))) in forall
-    (NEXT : next_state_updates st mvec [:: RegRead (inl r1) ; RegRead (inl r2) ; RegWrite (inl r3) (binop_denote (binop_of_binop op) w1 w2) ] = Some (st', ev)),
+    (NEXT : next_state_updates cde st mvec [:: RegRead (inl r1) ; RegRead (inl r2) ; RegWrite (inl r3) (binop_denote (binop_of_binop op) w1 w2) ] = Some (st', ev)),
       step cde st st' ev
 | step_load : forall mem reg pc tpc i ti r1 r2 w1 w2 t1 t2 old told 
     (ST   : st = State mem reg pc@tpc)
@@ -367,7 +349,7 @@ Inductive step (cde : code) (st st' : state) (ev : option event) : Prop :=
     (MEM1 : mem w1 = Some w2@t2)
     (OLD  : reg (to_nat r2) = Some old@told),
     let mvec := IVec tpc ti ([hseq t1; t2; told] : hseq _ (inputs LOAD)) in forall
-    (NEXT : next_state_updates st mvec [:: RegRead (inl r1) ; MemRead w1 ; RegWrite (inl r2) w2 ] = Some (st', ev)),
+    (NEXT : next_state_updates cde st mvec [:: RegRead (inl r1) ; MemRead w1 ; RegWrite (inl r2) w2 ] = Some (st', ev)),
     step cde st st' ev
 | step_store : forall mem reg pc i r1 r2 w1 w2 tpc ti t1 t2 old told
     (ST   : st = State mem reg pc@tpc)
@@ -377,7 +359,7 @@ Inductive step (cde : code) (st st' : state) (ev : option event) : Prop :=
     (R2W  : reg (to_nat r2) = Some w2@t2)
     (OLD  : mem w1 = Some old@told),
     let mvec := IVec tpc ti ([hseq t1; t2; told] : hseq _ (inputs STORE)) in forall
-    (NEXT : next_state_updates st mvec [:: RegRead (inl r1) ; RegRead (inl r2) ; MemWrite w1 w2 ] = Some (st', ev)),
+    (NEXT : next_state_updates cde st mvec [:: RegRead (inl r1) ; RegRead (inl r2) ; MemWrite w1 w2 ] = Some (st', ev)),
     step cde st st' ev
 | step_jump : forall mem reg pc i r w tpc ti t1
     (ST   : st = State mem reg pc@tpc)
@@ -385,7 +367,7 @@ Inductive step (cde : code) (st st' : state) (ev : option event) : Prop :=
     (INST : executing cde pc (MrJump r))
     (RW   : reg (to_nat r) = Some w@t1),
     let mvec := IVec tpc ti ([hseq t1] : hseq _ (inputs JUMP)) in forall
-    (NEXT : next_state_updates_and_pc st mvec [:: RegRead (inl r) ] w = Some (st', ev)),
+    (NEXT : next_state_updates_and_pc cde st mvec [:: RegRead (inl r) ] w = Some (st', ev)),
     step cde st st' ev
 | step_bnz : forall mem reg pc i r n w tpc ti t1
     (ST   : st = State mem reg pc@tpc)
@@ -393,8 +375,8 @@ Inductive step (cde : code) (st st' : state) (ev : option event) : Prop :=
     (INST : executing cde pc (MrBnz r n))
     (RW   : reg (to_nat r) = Some w@t1),
     let mvec := IVec tpc ti ([hseq t1] : hseq _ (inputs BNZ)) in
-     let pc' := word_of_nat (if w == 0%w then ((nat_of_word pc) + 1) else find_label cde n) in forall
-    (NEXT : next_state_updates_and_pc st mvec [:: RegRead (inl r) ] pc' = Some (st', ev)),
+    let optpc' := (if w == (word_of_nat 0) then Some ((nat_of_word (pc)) + 1) else find_label cde n) in forall pc' (PC' : optpc' = Some pc')
+    (NEXT : next_state_updates_and_pc cde st mvec [:: RegRead (inl r) ] (word_of_nat pc') = Some (st', ev)),
     step cde st st' ev
 | step_jal : forall mem reg pc i l tpc ti old told pc'
     (ST : st = State mem reg pc@tpc)
@@ -404,40 +386,43 @@ Inductive step (cde : code) (st st' : state) (ev : option event) : Prop :=
     (NOT_ALLOC : l <> alloc_label),
     let mvec := IVec tpc ti ([hseq told] : hseq _ (inputs JAL)) in
     forall (PC' :  Some pc' = (find_label cde l))
-    (NEXT : next_state_updates_and_pc st mvec [:: RegWrite (inl R_RA) (word_of_nat((nat_of_word pc).+1)) ] pc' = Some (st', ev)),
+    (NEXT : next_state_updates_and_pc cde st mvec [:: RegWrite (inl R_RA) (word_of_nat((nat_of_word pc).+1)) ] (word_of_nat pc') = Some (st', ev)),
     step cde st st' ev
-| step_jal_alloc : forall mem reg pc i l tpc ti old told
+| step_jal_alloc : forall mem reg pc i l tpc ti old told st_inter
     (ST : st = State mem reg pc@tpc)
     (PC : mem pc = Some i@ti)
     (INST : executing cde pc (MrJal l))
     (OLD : reg (to_nat R_RA) = Some old@told)
-    (ALLOC : l = alloc_label)
-    (ST' : (alloc_fun st) = Some st') (EV : ev = None),
+    (ALLOC : l = alloc_label),
+    let mvec := IVec tpc ti ([hseq told] : hseq _ (inputs JAL)) in
+    forall (NEXT : @next_state_do_update st Symbolic.R Other ( RegWrite (inl R_RA) (word_of_nat((nat_of_word pc).+1))) = Some st_inter)
+      (*NEXT : next_state_updates_and_pc cde st mvec [:: RegWrite (inl R_RA) (word_of_nat((nat_of_word pc).+1)) ] pc' = Some (st_inter, ev)*)
+    (ST' : (alloc_fun cde st_inter) = Some st') (EV : ev = None),
     step cde st st' ev
 .
 
 
 Definition eval_step (cde : code) (st : state) : option state_ev := 
-  let 'State mem reg pc@tpc := st in
+  let 'State mem reg pc@pctag := st in
   match (nth_error cde (nat_of_word pc)) with
   | None =>None
   | Some (instr,ti) =>
     match instr with
     | MrNop | MrLabel _ =>
-      let mvec := IVec tpc ti ([hseq] : hseq _ (inputs NOP)) in
-      next_state_updates st mvec [:: ]
+      let mvec := IVec pctag ti ([hseq] : hseq _ (inputs NOP)) in
+      next_state_updates cde st mvec [:: ]
     | MrConst n r =>
       do! old <- reg (to_nat r);
       let: _@told := old in
-      let ivec := IVec tpc ti ([hseq told] : hseq _ (inputs CONST)) in
-      next_state_updates st ivec [:: RegWrite (inl r) (swcast n)]
+      let ivec := IVec pctag ti ([hseq told] : hseq _ (inputs CONST)) in
+      next_state_updates cde st ivec [:: RegWrite (inl r) (swcast n)]
     | MrMov r1 r2 =>
       do! a1 <- reg (to_nat_bis r1);
       let: w1@t1 := a1 in
       do! a2 <- reg (to_nat_bis r2);
       let: _@told := a2 in
-      let mvec := IVec tpc ti ([hseq t1;told] : hseq _ (inputs MOV)) in
-      next_state_updates st mvec [:: RegRead r1 ; RegWrite r2 w1]
+      let mvec := IVec pctag ti ([hseq t1;told] : hseq _ (inputs MOV)) in
+      next_state_updates cde st mvec [:: RegRead r1 ; RegWrite r2 w1]
     | MrBinop op r1 r2 r3 =>
       do! a1 <- reg (to_nat r1);
       let: w1@t1 := a1 in
@@ -445,8 +430,8 @@ Definition eval_step (cde : code) (st : state) : option state_ev :=
       let: w2@t2 := a2 in
       do! a3 <- reg (to_nat r3);
       let: _@told := a3 in
-      let mvec := IVec tpc ti ([hseq t1;t2;told] : hseq _ (inputs (BINOP (binop_of_binop op)))) in
-      next_state_updates st mvec [:: RegRead (inl r1) ; RegRead (inl r2) ; RegWrite (inl r3) (binop_denote (binop_of_binop op) w1 w2)]
+      let mvec := IVec pctag ti ([hseq t1;t2;told] : hseq _ (inputs (BINOP (binop_of_binop op)))) in
+      next_state_updates cde st mvec [:: RegRead (inl r1) ; RegRead (inl r2) ; RegWrite (inl r3) (binop_denote (binop_of_binop op) w1 w2)]
     | MrLoad r1 r2 =>
       do! a1 <- reg (to_nat r1);
       let: w1@t1 := a1 in
@@ -454,8 +439,8 @@ Definition eval_step (cde : code) (st : state) : option state_ev :=
       let: w2@t2 := amem in
       do! a2 <- reg (to_nat r2);
       let: _@told := a2 in
-      let mvec := IVec tpc ti ([hseq t1;t2;told] : hseq _ (inputs LOAD)) in
-      next_state_updates st mvec [:: RegRead (inl r1) ; MemRead w1 ; RegWrite (inl r2) w2]
+      let mvec := IVec pctag ti ([hseq t1;t2;told] : hseq _ (inputs LOAD)) in
+      next_state_updates cde st mvec [:: RegRead (inl r1) ; MemRead w1 ; RegWrite (inl r2) w2]
     | MrStore r1 r2 =>
       do! a1 <- reg (to_nat r1);
       let: w1@t1 := a1 in
@@ -463,32 +448,45 @@ Definition eval_step (cde : code) (st : state) : option state_ev :=
       let: _@told := amem in
       do! a2 <- reg (to_nat r2);
       let: w2@t2 := a2 in
-      let mvec := IVec tpc ti ([hseq t1;t2;told] : hseq _ (inputs STORE)) in
-      next_state_updates st mvec [:: RegRead (inl r1) ; RegRead (inl r2) ; MemWrite w1 w2]
+      let mvec := IVec pctag ti ([hseq t1;t2;told] : hseq _ (inputs STORE)) in
+      next_state_updates cde st mvec [:: RegRead (inl r1) ; RegRead (inl r2) ; MemWrite w1 w2]
     | MrJump r =>
       do! a <- reg (to_nat r);
       let: w@t1 := a in
-      let mvec := IVec tpc ti ([hseq t1] : hseq _ (inputs JUMP)) in
-      next_state_updates_and_pc st mvec [:: RegRead (inl r)] w
+      let mvec := IVec pctag ti ([hseq t1] : hseq _ (inputs JUMP)) in
+      next_state_updates_and_pc cde st mvec [:: RegRead (inl r)] w
     | MrBnz r n =>
       do! a <- reg (to_nat r);
       let: w@t1 := a in
-      let pc' := word_of_nat (if w == 0%w then ((nat_of_word pc) + 1) else find_label cde n) in
-      let ivec := IVec tpc ti ([hseq t1] : hseq _ (inputs BNZ)) in
-      next_state_updates_and_pc st ivec [:: RegRead (inl r)] pc'
+      do! pc' <- (if w == (word_of_nat 0) then Some ((nat_of_word (pc)) + 1) else find_label cde n);
+      let ivec := IVec pctag ti ([hseq t1] : hseq _ (inputs BNZ)) in
+      next_state_updates_and_pc cde st ivec [:: RegRead (inl r)] (word_of_nat pc')
     | MrJal i =>
-      if (eqn i alloc_label) then
-        do! st' <- alloc_fun st;
-        Some (st, None)
+        if (eqn i alloc_label) then
+        do! st_inter <- (@next_state_do_update st Symbolic.R Other ( RegWrite (inl R_RA) (word_of_nat((nat_of_word pc).+1))));
+        do! st' <- alloc_fun cde st_inter;
+        Some (st', None)
       else
       do! oldtold <- reg (to_nat R_RA);
       let: _@told := oldtold in
-      let mvec := IVec tpc ti ([hseq told] : hseq _ (inputs JAL)) in
+      let mvec := IVec pctag ti ([hseq told] : hseq _ (inputs JAL)) in
       match (find_label cde i) with
       | None => None
-      | Some (pc') => next_state_updates_and_pc st mvec [:: RegWrite (inl R_RA) (word_of_nat((nat_of_word pc).+1))] pc'
+      | Some (pc') => next_state_updates_and_pc cde st mvec [:: RegWrite (inl R_RA) (word_of_nat((nat_of_word pc).+1))] (word_of_nat pc')
       end
     | MrHalt => None
+    end
+  end.
+
+Fixpoint execN (n: nat) (cde: code) (st: state) : option Z + nat :=
+  match n with
+  | O => inr 3
+  | S n' =>
+    match eval_step cde st with
+    | None => (inl (
+             do! w <- (regs st (to_nat R_COM));
+             Some (Symbolic.convert (word.int_of_word (vala w)))))
+    | Some (st', _) => execN n' cde st'
     end
   end.
 
@@ -512,16 +510,29 @@ Fixpoint fold_left_map {FROM ACC TO: Type} (f : ACC -> FROM -> TO * ACC) (init :
   | cons e ll => let (val,acc) := (f init e) in val :: (fold_left_map f acc ll)
 end.
 
-Search (nat -> nat -> nat).
+Fixpoint fold_left_map_bis {FROM ACC TO: Type} (f : ACC -> FROM -> TO * ACC) (init : ACC) (l : list FROM) : (list TO) * ACC :=
+  match l with
+  | nil => (nil, init)
+  | cons e ll => let (val,acc) := (f init e) in let (res, a) := (fold_left_map_bis f acc ll) in (val :: res, a)
+end.
 
 (* code_lengths cde c give you the line at which the code of the compartment c begins*)
-Definition code_lengths (cde : Transitional.code) : NMap nat :=
-  (* this take into account the fact that the allocation is linearized into 5 instructions *)
-  let size_instr := (fun (i:Transitional.instr) => match i with | TrAlloc _ _ => 5 | _ => 1 end) in
-  let size_sum := (fold_left (fun n (im : Transitional.instr * Transitional.mem_tag) => let (i,_) := im in n + (size_instr i)) 0) in
-  let l := Maps.elementsm (mapm size_sum cde) in
-  mkfmap (fold_left_map (fun (count : nat) (p:nat*nat) => let (color, size) := p in ((color,count), count+size)) 0 l).
+Definition memory_lengths (buf : NMap {fmap Block.id -> nat + seq value}):  NMap (NMap nat) :=
+  (*
+  (* this (notably) takes into account the fact that the allocation is linearized into 5 instructions *)
+  let size_instr := (fun (i:Transitional.instr) => match i with | TrAlloc _ _ => 5 | TrLabel (_,Some _) => 2 | _ => 1 end) in
+  let size_sum := (fold_left (fun n im => n + 1) 0) in
+  let l := Maps.elementsm (mapm (fun m => mkfmap (size_sum (Maps.elementsm m))) buf) in
+  mkfmap (fold_left_map (fun (count : nat) (p:nat*nat) => let (color, size) := p in ((color,count), count+size)) 0 l).*)
 
+  let l := Maps.elementsm (mapm Maps.elementsm buf) in (* turns fmaps into lists *)
+  let f := (fun acc => fold_left_map_bis (fun acc' (a : nat * (nat + seq value)) =>
+                                     match (snd a) with
+                                      | inl n => ((fst a, acc'), n + acc')
+                                      | inr s => ((fst a, acc'), (size s) + acc') end
+                      ) acc) in
+  mkfmap (fold_left_map (fun acc s => let (flat,count) := f acc (snd s) in
+                           ((fst s, mkfmap (flat)), count + acc) ) 0 l).
 
 
 Definition encode_int (z : Z) : ssrint.int :=
@@ -531,20 +542,23 @@ Definition encode_int (z : Z) : ssrint.int :=
   | Z.neg n => ssrint.Negz (ssrnat.nat_of_pos n)
   end.
 
-Definition convert_value (cde_l : NMap nat) (iv : imvalue) : imm mt :=
+Definition convert_value (memory_size : NMap (NMap nat)) (iv : imvalue) : imm mt :=
   match iv with
   | IInt z => word.as_word (encode_int z)
-  | IPtr p => match (cde_l (Pointer.component p)) with
-             | None => (word.as_word (ssrint.Posz 0))
-             | Some s => let z := Z.add (Z.of_nat s) (Pointer.offset p) in word.as_word (encode_int z) end                         
+  | IPtr p => word_of_nat
+      (Option.default (0)
+         (do! map <- (memory_size (Pointer.component p));
+          do! s <- (map :NMap nat) (Pointer.block p);
+          Some (Z.to_nat (Z.add (Z.of_nat s) (Pointer.offset p)))))
   end.
 
 
-Definition instr_translation (cde_l : NMap nat) (i : Transitional.instr) : (seq instr) :=
+Definition instr_translation (make_label : proc_label -> nat) (update_label : nat -> nat) (memory_size : NMap (NMap nat)) (i : Transitional.instr) : (seq instr) :=
   match i with
     | TrNop => MrNop :: nil
-    | TrLabel (l, _) => MrLabel l :: nil
-    | TrConst iv reg => MrConst (convert_value cde_l iv) reg :: nil
+    | TrLabel (l, None) => MrLabel (update_label l) :: nil
+    | TrLabel (l, Some pl) => MrLabel (update_label l) :: (MrLabel (make_label pl)) :: nil
+    | TrConst iv reg => MrConst (convert_value memory_size iv) reg :: nil
     | TrMov r1 r2 => MrMov (inl r1) (inl r2) :: nil
     | TrBinOp b r1 r2 r3 => MrBinop b r1 r2 r3 :: nil
     | TrLoad r1 r2 => MrLoad r1 r2 :: nil
@@ -555,24 +569,98 @@ Definition instr_translation (cde_l : NMap nat) (i : Transitional.instr) : (seq 
                              (MrJal alloc_label)  ;
                              (MrMov (inr R_SC_ARG3) (inl R_RA))  ;
                              (MrMov (inr R_SC_RET) (inl rptr))] in l 
-    | TrBnz r l => MrBnz r l :: nil
+    | TrBnz r l => MrBnz r (update_label l) :: nil
     | TrJump r => MrJump r :: nil
-    | TrJalNat l => MrJal l :: nil
-    | TrJalProc (l,_) => MrJal (l) :: nil
+    | TrJalNat l => MrJal (update_label l) :: nil
+    | TrJalProc pl => MrJal (make_label pl) :: nil
     | TrHalt => MrHalt :: nil
   end.
 
-Definition transitional_to_merged (cde : Transitional.code) : code :=
-  let cde_l := code_lengths cde in
-  let f := fun (c: code) (itrt: Transitional.instr * mem_tag) =>
-             let (itr, t) := itrt in
-             let il := map (fun i => (i,t)) (instr_translation cde_l itr) in cat il c in
-  let add_color := (fun (c:Component.id) (p:Transitional.instr * Transitional.mem_tag) =>
-                      let (i, t) := p in (i, {| vtag := Transitional.vtag t ;
-                                                color := c ;
-                                                entry := Transitional.entry t |})) in
-  let add_color_l := (fun (p:(nat * seq (Transitional.instr * Transitional.mem_tag)))=>
-                      let (c, l) := p in map (add_color c) l) in
-  let c :=  flatten(map add_color_l  (Maps.elementsm cde)) in
-  fold_right f nil c.
+Definition transitional_to_merged (p: Intermediate.program) (cde : Transitional.code) : code :=
+  let memory_size := memory_lengths (Intermediate.prog_buffers p) in
+  let max_seq := (fun l => foldl Init.Nat.max 0 (map (fun p => match (fst p) with | TrLabel (la,_) => la | _ => 0 end) l )) in
+  let lmax := foldl Init.Nat.max 0 (codomm(mapm max_seq cde)) in
+  let max_seq := (fun l => foldl Init.Nat.max 0 (map (fun p => match (fst p) with | TrLabel (_,Some(_,p)) => p | _ => 0 end) l )) in
+  let pmax := foldl Init.Nat.max 0 (codomm(mapm max_seq cde)) in
+  let cmax := foldl Init.Nat.max 0 (domm cde) in
+  let make_label := (fun pl => lmax * (cmax + 1) + 1 + (fst pl)*pmax + (snd pl)) in
+  let update_label := (fun c old => old + lmax * (c)) in
+  let f := (fun  (itrt: Transitional.instr * mem_tag) (c: code) =>
+    let (itr, t) := itrt in
+    let il := map (fun i => (i,t)) (instr_translation make_label (update_label (color t)) memory_size itr) in app il c) in
+  let c :=  flatten(map snd  (Maps.elementsm cde)) in
+  foldr f nil c.
+
+Definition inital_memory (p : Intermediate.program) :=
+  let p := Linearize.linearize p in
+  let bufs := Linearize.buffers p in
+    let base_adress c b :=
+     (*  length of code + 1 + number of triples (c',b',_) such that (c', b') that occur before (c, b) *)
+      (*length (Linearize.procedures p) + 1 +*)
+      length (domm (filterm (fun x _ => match x with (c', b', _) => (c' < c) || ((c' == c) && (b' < b)) end)
+                     (* TL TODO codomm doesn't typecheck... *)
+                     (* Invariant: Linearize.buffers is "continuous" *)
+                     ((Linearize.buffers p))))
+  in
+  let concretize := (fun p => match p with
+                              | (c, b, o) =>
+                                (* TL TODO: I have add notation issues, hence intZmod.addz... *)
+                                ssrint.intZmod.addz (encode_int o) (ssrint.Posz (base_adress c b))
+                              end) in
+  let f (x : nat * nat * nat) : mword mt :=
+    match x with (c, b, o) => word.as_word (concretize (c, b, Z.of_nat o)) end in
+  let encode_memval : ((value * mem_tag) -> (atom mem_tag)) := (fun x =>
+  {| vala := match fst x with
+             | Int z => word.as_word (encode_int z)
+             | Ptr p => word.as_word (concretize p)
+             | Undef =>  word.as_word (ssrint.Posz 0) (* Invariant: should not be present *)
+             end ;
+     taga := snd x |})
+  in Tmp.mapk f (mapm (encode_memval) bufs).
+
+Definition run_merged cd mem0 fuel :=
+  let default_reg := (word_of_nat 0)@(LRC.Other): atom (tag_type Symbolic.R) in
+  let reg0 := [fmap (0, default_reg) ;
+               (1, default_reg) ;
+               (2, default_reg) ;
+               (3, default_reg) ;
+               (4, (word_of_nat (1+size cd))@(LRC.Other)) ; (* value equivalent to "Undef" for R_RA*)
+               (5, default_reg) ;
+               (6, default_reg) ;
+               (16,default_reg) ;
+               (17,default_reg) ;
+               (18,default_reg) ;
+               (19,default_reg) ] in
+  let pctag := build_tpc 0 in
+      execN fuel cd {|mem := mem0 ; regs := reg0 ; pc := (word_of_nat 0)@pctag|}.
+
+
+Definition compile_run_merged fuel (p : Intermediate.program) :=
+ run_merged (transitional_to_merged p (pre_linearize p)) (inital_memory p) fuel .
+
+Close Scope monad_scope.
+
+
+Definition compile_and_run_from_source_merged := 
+fun (p : Source.program) (fuel : nat) =>
+match Compiler.compile_program p with
+| Some compiled_p => compile_run_merged fuel compiled_p
+| None => inl None
+end.
+
+End WithClasses.
+
+
+Definition compile_and_run_from_source_merged_ex (mt : machine_types) := 
+fun (p : Source.program) (fuel : nat) =>
+match Compiler.compile_program p with
+| Some compiled_p =>
+    match @compile_run_merged mt fuel compiled_p with
+    | inl (Some n) => print_ocaml_int (z2int n)
+    | inl None => print_error ocaml_int_1
+    | inr n => print_error (nat2int n)
+    end
+| None => print_error ocaml_int_0
+end.
+
 
