I2MP/Examples/Identity.v
@@ -3,8 +3,18 @@ Require Import Common.Values.
 Require Import Transitional.
 Require Import Source.Examples.Identity.
 
-Definition fuel := 1000%nat.
+Definition fuel := 200%nat.
 Definition to_run := compile_and_run_from_source_ex identity fuel.
 
 Set Warnings "-extraction-reserved-identifier".
 Extraction "/tmp/run_mp_compiled_identity.ml" to_run.
+
+
+Require Import Merged Int32.
+
+Definition to_run_mr := @Merged.compile_and_run_from_source_merged_ex concrete_int_32_mt identity fuel.
+(*
+Definition to_run_mr := @I2MP.Examples.Helper.compile_and_run_and_show_from_source_merged concrete_int_32_mt identity fuel.
+*)
+Set Warnings "-extraction-reserved-identifier".
+Extraction "/tmp/run_merged_compiled_identity.ml" to_run_mr.
