I2MP/Examples/Increment.v
@@ -8,3 +8,11 @@ Definition to_run := compile_and_run_from_source_ex increment fuel.
 
 Set Warnings "-extraction-reserved-identifier".
 Extraction "/tmp/run_mp_compiled_increment.ml" to_run.
+
+Require Import Merged Int32 I2MP.Examples.Helper.
+
+Definition to_run_mr := @Merged.compile_and_run_from_source_merged_ex concrete_int_32_mt increment fuel.
+(*
+Definition to_run_mr := @I2MP.Examples.Helper.compile_and_run_and_show_from_source_merged concrete_int_32_mt increment fuel. *)
+Set Warnings "-extraction-reserved-identifier".
+Extraction "/tmp/run_merged_compiled_increment.ml" to_run_mr.
