I2MP/Examples/NestedCalls.v
@@ -10,3 +10,11 @@ Definition to_show := compile_and_show nested_calls.
 
 Set Warnings "-extraction-reserved-identifier".
 Extraction "/tmp/run_mp_compiled_nested_calls.ml" to_run.
+
+Require Import Merged Int32 I2MP.Examples.Helper.
+
+Definition to_run_mr := @Merged.compile_and_run_from_source_merged_ex concrete_int_32_mt nested_calls fuel.
+(*
+Definition to_run_mr := @I2MP.Examples.Helper.compile_and_run_and_show_from_source_merged concrete_int_32_mt nested_calls fuel. *)
+Set Warnings "-extraction-reserved-identifier".
+Extraction "/tmp/run_merged_compiled_nested_calls.ml" to_run_mr.
