run_extracted_examples.sh
@@ -7,6 +7,7 @@ SOURCE_PREFIX="run_source_"
 INTERMEDIATE_PREFIX="run_intermediate_compiled_"
 TARGET_PREFIX="run_target_compiled_"
 MP_PREFIX="run_mp_compiled_"
+MERGED_PREFIX="run_merged_compiled_"
 
 if (( $# == 1 )); then
     if [[ $1 = "--force-extraction" ]]; then
@@ -58,6 +59,17 @@ done
 # run compiled examples at the micro-policy level
 echo "*** Examples compiled at the micro-policy level ***"
 for example in $MP_PREFIX*.ml; do
+    [ -f "$example" ] || continue
+    # prepend big int import to each example
+    echo -e "open Big_int\n$(cat $example)" > $example
+    echo "Output of $example:"
+    ocaml nums.cma big.cma $example
+done
+
+
+# run compiled examples at the "merged" level
+echo "*** Examples compiled at the merged level ***"
+for example in $MERGED_PREFIX*.ml; do
     [ -f "$example" ] || continue
     # prepend big int import to each example
     echo -e "open Big_int\n$(cat $example)" > $example
